---
title: "CFerrari_Assignment14"
author: "Charley Ferrari"
date: "Thursday, May 07, 2015"
output: pdf_document
---

$$f(x) = \frac{1}{1-x}$$

$$f(x) = \sum_{n=0}^{\infty}  \frac{f^{(n)} (a)}{n!} (x-a)^n$$

Lets first try to arrive at a general derivative form for $\frac{1}{1-x}$

$$f^{(1)}(x) = (-1)(-1) \frac{1}{(1-x)^2}$$

$$f^{(2)}(x) = (-1)^2 (-1)(-2) \frac{1}{(1-x)^3}$$

$$f^{(3)}(x) = (-1)^3 (-1)(-2)(-3) \frac{1}{(1-x)^4}$$

The negative terms always cancel eachother out

$$f^{(n)}(x) = \frac{1}{n!(1-x)^{n+1}}$$

The n! terms cancel eachother out:

$$\frac{1}{1-x} = \sum_{n=0}^{\infty} \frac{(-1)^{n+1} (x-a)^n}{(1-a)^{n+1}}$$

So for a = 0:

$$\frac{1}{1-x} = \sum_{n=0}^{\infty} x^n$$

And since this is a basic power series, the radius of convervence is -1 < x < 1, since the 
$\lim_{x\to\infty} p^x$ is 0 for that radius.

-----------------------------------

$$f(x) = e^x$$

The multiple derivatives of this is easy, $\frac{d}{dx} e^x$ is just $e^x$

$$e^x = \sum_{n=0}^{\infty} \frac{e^a}{n!} (x-a)^n$$

Lets take a = 0

$$e^x = \sum_{n=0}^{\infty} \frac{x^n}{n!}$$

Lets try to find its radius of convergence by using the ratio test.

$$\frac{A_{n+1}}{A_n} = \frac{x^{n+1}}{(n+1)n!} \frac{n!}{x^n} = \frac{x}{n+1}$$

$$\lim_{x\to\infty} \frac{x}{n+1} = 0$$

No matter what value x takes, the ratio converges to 0, so the series converges for all values of x

-----------------------------------

$$f(x) = ln(1+x)$$

Lets first try to arrive at a general derivative form for $ln(1+x)$

$$f(x) = ln(1+x)$$

$$f^{(1)}(x) = \frac{1}{1+x}$$

$$f^{(2)}(x) = (-1) \frac{1}{(1+x)^2}$$

$$f^{(3)}(x) = (-1)(-2) \frac{1}{(1+x)^3}$$

$$f^{(n)}(x) = (-1)^{n-1} (n-1)! \frac{1}{(1+x)^n}$$

$\frac{(n-1)!}{n!} = \frac{1}{n}$, so, for a=0:

$$ln(1+x) = \sum_{n=0}^{\infty} -1^{n-1} \frac{x^n}{n}$$

Lets try to find its radius of convergence by using the ratio test.

$$\frac{A_{n+1}}{A_n} = - \frac{x^{n+1}}{n} \frac{n}{x^n} = - \frac{xn}{n+1}$$

$$\lim_{n\to\infty} - \frac{xn}{n+1} = -x$$

So, this is valid when $|x| < 1$